src/AtomicRules.v
@@ -1,0 +1,21 @@
+Require Import Bool List String Peano_dec.
+Require Import Common ListSupport FMap Syntax Semantics StepDet Serial.
+Require Import Synthesis TrsInv TrsSim.
+
+(* Lemma what_we_want_using_atomic_rules: *)
+(*   forall impl ti hst mouts orsout, *)
+(*     Atomic impl ti (ilbl :: hst) mouts orsout -> *)
+(*     forall pist ist1, *)
+(*       steps_det impl pist hst ist1 -> *)
+(*       step_det impl ist1 ilbl ist2 -> *)
+(*       AtomicRules impl trsIdx rqin rqs .. *)
+
+Section AtomicRules.
+
+  Variables
+    (impl: System)
+    (trsIdx: IdxT)
+    (rqin: Msg).
+
+End AtomicRules.
+
